disk-betree/ImplModelLeaf.i.dfy
@@ -40,8 +40,7 @@ module ImplModelLeaf {
     if (!(s.frozenIndirectionTable.Some? && ref in IIndirectionTable(s.frozenIndirectionTable.value).graph ==> ref in IIndirectionTable(s.frozenIndirectionTable.value).locs)) then (
       s
     ) else (
-      var joined := KMTable.join(node.buckets);
-      KMTable.joinEqJoinBucketList(node.buckets, node.pivotTable);
+      var joined := KMTable.join(node.buckets, node.pivotTable);
 
       var pivots := GetNewPivots(joined);
 
